wip

test/address_properties/main.c
@@ -1,0 +1,334 @@
+#include <assert.h>
+#include <stdbool.h>
+#include <stdint.h>
+#include <stdio.h>
+#include <stdlib.h>
+#include <string.h>
+
+#include "randombytes.h"
+#include "wots.h"
+#include "xmss_commons.h"
+
+#define str(s) #s
+#define xstr(s) str(s)
+
+#ifndef IMPL
+#error IMPL not defined
+#endif
+
+static int starts_with(const char *str, const char *prefix) { return strncmp(str, prefix, strlen(prefix)) == 0; }
+
+static void flip_addr(uint32_t *a, size_t idx) {
+    assert(a != NULL);
+    assert(idx < 8);
+
+    a[idx] ^= 0xFFFFFFFF;
+}
+
+static void print_diff_addr(const char *impl, const uint32_t *before, const uint32_t *after) {
+    assert(impl != NULL);
+    assert(before != NULL);
+    assert(after != NULL);
+
+    for (size_t i = 0; i < 8; i++) {
+        if (before[i] != after[i]) {
+            printf("[%s:] index %ld was changed: value = %d\n", impl, i, after[i]);
+        }
+    }
+}
+
+void test_pre_wots_pk_gen(const xmss_params *p) {
+    assert(p != NULL);
+
+    uint8_t pub_seed[p->n], sk_seed[p->n];
+    uint8_t pk0[p->wots_sig_bytes], pk1[p->wots_sig_bytes];
+    uint32_t addr0[8], addr1[8];
+
+    randombytes(pub_seed, p->n * sizeof(uint8_t));
+    randombytes(sk_seed, p->n * sizeof(uint8_t));
+
+    for (size_t i = 0; i < 8; i++) {
+        memset(pk0, 0, p->wots_sig_bytes);
+        memset(pk1, 0, p->wots_sig_bytes);
+
+        randombytes((uint8_t *)addr0, 8 * sizeof(uint32_t));
+        memcpy(addr1, addr0, 8 * sizeof(uint32_t));
+
+        assert(!memcmp(addr0, addr1, 8 * sizeof(uint32_t)));
+
+        flip_addr(addr1, i);
+
+        assert(addr0[i] != addr1[i]);
+
+        for (size_t j = 0; j < 8; j++) {
+            if (j != i) {
+                assert(addr0[j] == addr1[j]);
+            }
+        }
+
+        wots_pkgen(p, pk0, sk_seed, pub_seed, addr0);
+        wots_pkgen(p, pk1, sk_seed, pub_seed, addr1);
+
+        if (!memcmp(pk0, pk1, p->wots_sig_bytes) && true) {
+            printf("[wots_pkgen]: Changing index %ld of the address does not change the result\n", i);
+        }
+
+        if (memcmp(pk0, pk1, p->wots_sig_bytes) && false) {
+            printf("[wots_pkgen]: Changing index %ld of the address changes the result\n", i);
+        }
+    }
+}
+
+void test_pre_expand_seed(const xmss_params *p) {
+    assert(p != NULL);
+
+    uint8_t pub_seed[p->n], sk_seed[p->n];
+    uint8_t pk0[p->wots_sig_bytes], pk1[p->wots_sig_bytes];
+    uint32_t addr0[8], addr1[8];
+
+    randombytes(pub_seed, p->n * sizeof(uint8_t));
+    randombytes(sk_seed, p->n * sizeof(uint8_t));
+
+    for (size_t i = 0; i < 8; i++) {
+        memset(pk0, 0, p->wots_sig_bytes);
+        memset(pk1, 0, p->wots_sig_bytes);
+
+        randombytes((uint8_t *)addr0, 8 * sizeof(uint32_t));
+        memcpy(addr1, addr0, 8 * sizeof(uint32_t));
+
+        assert(!memcmp(addr0, addr1, 8 * sizeof(uint32_t)));
+
+        flip_addr(addr1, i);
+
+        assert(addr0[i] != addr1[i]);
+
+        for (size_t j = 0; j < 8; j++) {
+            if (j != i) {
+                assert(addr0[j] == addr1[j]);
+            }
+        }
+
+        expand_seed(p, pk0, sk_seed, pub_seed, addr0);
+        expand_seed(p, pk1, sk_seed, pub_seed, addr1);
+
+        if (!memcmp(pk0, pk1, p->wots_sig_bytes) && true) {
+            printf("[expand_seed]: Changing index %ld of the address does not change the result\n", i);
+        }
+
+        if (memcmp(pk0, pk1, p->wots_sig_bytes) && false) {
+            printf("[expand_seed]: Changing index %ld of the address changes the result\n", i);
+        }
+    }
+}
+
+void test_pre_gen_chain_inplace(const xmss_params *p) {
+    assert(p != NULL);
+
+    uint8_t pub_seed[p->n], sk_seed[p->n];
+    uint8_t buf0[p->n], buf1[p->n];
+    uint32_t addr0[8], addr1[8];
+    uint32_t start, steps;
+
+    do {
+        randombytes((uint8_t *)&start, sizeof(uint32_t));
+        randombytes((uint8_t *)&steps, sizeof(uint32_t));
+    } while (start + steps >= p->wots_w);
+
+    if (start > steps) {
+        uint32_t temp = start;
+        start = steps;
+        steps = temp;
+    }
+
+    assert(start + steps <= p->wots_w - 1);
+
+    randombytes(pub_seed, p->n * sizeof(uint8_t));
+    randombytes(sk_seed, p->n * sizeof(uint8_t));
+
+    for (size_t i = 0; i < 8; i++) {
+        randombytes(buf0, p->n);
+        randombytes(buf1, p->n);
+
+        randombytes((uint8_t *)addr0, 8 * sizeof(uint32_t));
+        memcpy(addr1, addr0, 8 * sizeof(uint32_t));
+
+        assert(!memcmp(addr0, addr1, 8 * sizeof(uint32_t)));
+
+        flip_addr(addr1, i);
+
+        assert(addr0[i] != addr1[i]);
+
+        for (size_t j = 0; j < 8; j++) {
+            if (j != i) {
+                assert(addr0[j] == addr1[j]);
+            }
+        }
+
+        gen_chain(p, buf0, buf0, start, steps, pub_seed, addr0);
+        gen_chain(p, buf1, buf1, start, steps, pub_seed, addr1);
+
+        if (!memcmp(buf0, buf1, p->n) && true) {
+            printf("[gen_chain]: Changing index %ld of the address does not change the result\n", i);
+        }
+
+        if (memcmp(buf0, buf1, p->n) && true) {
+            printf("[gen_chain]: Changing index %ld of the address changes the result\n", i);
+        }
+    }
+}
+
+void test_pre_ltree(const xmss_params *p) {
+    assert(p != NULL);
+
+    uint8_t pub_seed[p->n];
+    uint8_t leaf0[p->n], leaf1[p->n];
+    uint8_t wots_pk0[p->wots_sig_bytes], wots_pk1[p->wots_sig_bytes];
+    uint32_t addr0[8], addr1[8];
+
+    randombytes(pub_seed, p->n * sizeof(uint8_t));
+
+    for (size_t i = 0; i < 8; i++) {
+        memset(leaf0, -1, p->n);
+        memset(leaf1, -1, p->n);
+
+        randombytes(wots_pk0, p->wots_sig_bytes);
+        memcpy(wots_pk1, wots_pk0, p->wots_sig_bytes);
+        assert(!memcmp(wots_pk0, wots_pk1, p->wots_sig_bytes));
+
+        randombytes((uint8_t *)addr0, 8 * sizeof(uint32_t));
+        memcpy(addr1, addr0, 8 * sizeof(uint32_t));
+
+        assert(!memcmp(addr0, addr1, 8 * sizeof(uint32_t)));
+
+        flip_addr(addr1, i);
+
+        assert(addr0[i] != addr1[i]);
+
+        for (size_t j = 0; j < 8; j++) {
+            if (j != i) {
+                assert(addr0[j] == addr1[j]);
+            }
+        }
+
+        l_tree(p, leaf0, wots_pk0, pub_seed, addr0);
+        l_tree(p, leaf0, wots_pk1, pub_seed, addr1);
+
+        if (!memcmp(leaf0, leaf1, p->n) && !memcmp(wots_pk0, wots_pk1, p->wots_sig_bytes)) {
+            printf("[l_tree]: Changing index %ld of the address does not change the result\n", i);
+        }
+
+        if (memcmp(leaf0, leaf1, p->n) || memcmp(wots_pk0, wots_pk1, p->wots_sig_bytes)) {
+            printf("[l_tree]: Changing index %ld of the address changes the result\n", i);
+        }
+    }
+}
+
+void test_pre(const xmss_params *p) {
+    assert(p != NULL);
+
+    test_pre_wots_pk_gen(p);
+    // test_pre_expand_seed(p);
+    // test_pre_gen_chain_inplace(p);
+    // test_pre_ltree(p);
+}
+
+void test_post_wots_pk_gen(const xmss_params *p) {
+    assert(p != NULL);
+
+    uint8_t pub_seed[p->n], sk_seed[p->n];
+    uint8_t pk[p->wots_sig_bytes];
+    uint32_t addr_before[8], addr_after[8];
+
+    randombytes(pub_seed, p->n * sizeof(uint8_t));
+    randombytes(sk_seed, p->n * sizeof(uint8_t));
+    memset(addr_before, -1, 8 * sizeof(uint32_t));
+    memcpy(addr_after, addr_before, 8 * sizeof(uint32_t));
+    assert(!memcmp(addr_before, addr_after, 8 * sizeof(uint32_t)));
+    wots_pkgen(p, pk, sk_seed, pub_seed, addr_after);
+    print_diff_addr("wots pk gen", addr_before, addr_after);
+}
+
+void test_post_expand_seed(const xmss_params *p) {
+    uint8_t buf0[p->n], buf1[p->n];
+    uint8_t pk[p->wots_sig_bytes];
+    uint32_t addr_before[8], addr_after[8];
+
+    randombytes(buf0, p->n * sizeof(uint8_t));
+    randombytes(buf1, p->n * sizeof(uint8_t));
+
+    // Post: addr[5] = len - 1 /\ addr[6] = 0 /\ addr[7] = 0
+    memset(addr_before, -1, 8 * sizeof(uint32_t));
+    memcpy(addr_after, addr_before, 8 * sizeof(uint32_t));
+    assert(!memcmp(addr_before, addr_after, 8 * sizeof(uint32_t)));
+    expand_seed(p, pk, buf0, buf1, addr_after);
+    print_diff_addr("expand seed", addr_before, addr_after);
+}
+
+void test_post_gen_chain(const xmss_params *p) {
+    assert(p != NULL);
+
+    uint8_t buf0[p->n], buf1[p->n];
+    uint32_t addr_before[8], addr_after[8];
+
+    randombytes(buf0, p->n * sizeof(uint8_t));
+    randombytes(buf1, p->n * sizeof(uint8_t));
+
+    // Post: addr[6] = MIN (start + steps - 1, w - 1) /\ addr[7] = 1
+    memset(addr_before, -1, 8 * sizeof(uint32_t));
+    memcpy(addr_after, addr_before, 8 * sizeof(uint32_t));
+    assert(!memcmp(addr_before, addr_after, 8 * sizeof(uint32_t)));
+    gen_chain(p, buf0, buf0, 0, 10, buf1, addr_after);
+    print_diff_addr("gen_chain_inplace", addr_before, addr_after);
+}
+
+void test_post_l_tree(const xmss_params *p) {
+    assert(p != NULL);
+
+    uint8_t pub_seed[p->n];
+    uint8_t leaf[p->n];
+    uint8_t wots_pk[p->wots_sig_bytes];
+    uint32_t addr_before[8], addr_after[8];
+
+    randombytes(pub_seed, p->n * sizeof(uint8_t));
+    randombytes(wots_pk, p->wots_sig_bytes);
+    memset(addr_before, -1, 8 * sizeof(uint32_t));
+    memcpy(addr_after, addr_before, 8 * sizeof(uint32_t));
+    assert(!memcmp(addr_before, addr_after, 8 * sizeof(uint32_t)));
+
+    l_tree(p, leaf, wots_pk, pub_seed, addr_after);
+    print_diff_addr("l_tree", addr_before, addr_after);
+}
+
+void test_post(const xmss_params *p) {
+    assert(p != NULL);
+
+    test_post_wots_pk_gen(p);
+    // test_post_expand_seed(p);
+    // test_post_gen_chain(p);
+    // test_post_l_tree(p);
+}
+
+int main(void) {
+    xmss_params p;
+    uint32_t oid;
+
+    if (!starts_with(xstr(IMPL), "XMSSMT")) {
+        puts("THIS ONLY WORKS FOR THE MULTI TREE VARIANT");
+        return -1;
+    }
+
+    if (xmssmt_str_to_oid(&oid, xstr(IMPL)) == -1) {
+        fprintf(stderr, "Failed to generate oid from impl name\n");
+        return -1;
+    }
+
+    if (xmssmt_parse_oid(&p, oid) == -1) {
+        fprintf(stderr, "Failed to generate params from oid\n");
+        return -1;
+    }
+
+    test_pre(&p);
+    test_post(&p);
+
+    return 0;
+}
