proof/correctness/Repr2.ec
@@ -117,6 +117,9 @@ op DecodeWotsSk (sk : wots_sk) : W8.t Array2144.t =
 op DecodeWotsPk (pk : wots_pk) : W8.t Array2144.t = 
   Array2144.of_list witness (nbytes_flatten (val pk)).
 
+op EncodeWotsPk (pk : W8.t Array2144.t) : wots_pk = 
+  LenNBytes.insubd (map NBytes.insubd (chunk n (to_list pk))).
+
 op EncodeWotsSignature (s : W8.t Array2144.t) : wots_signature = 
   LenNBytes.insubd (map NBytes.insubd (chunk 32 (to_list s))). 
 
