proof/correctness/test.ec
@@ -1,0 +1,6 @@
+require import AllCore.
+
+lemma test : forall x y, x + 2 * y <= 4 && 2 * x + y <= 4 => x + y < 3.
+proof.
+coq edit "test" ().
+qed.
