proof/spec/xmss/XMSS_Types.ec
@@ -8,9 +8,16 @@ from Jasmin require import JModel.
 require import Types Array8 LTree.
 import Params.
 
+clone export Subtype as AuthPath with
+  type T = nbytes list,
+  op P = fun l => size l = h (* Section 4.1.8. of the RFC *)
+                             (* The size is h / d for the multi tree variant *)
+  rename "sT" as "auth_path"
+  proof inhabited by (exists (nseq h witness);smt(size_nseq ge0_h))
+  proof *.
+
 type sig_t = { sig_idx : W32.t;
                r : nbytes ;
                r_sig : (wots_signature * auth_path) }.
-
 
 (******************************************************************************)
