README.md
@@ -1,2 +1,25 @@
 # xmss-jasmin
 
+- XMSSMT-SHA2_20/2_256
+
+```
+[partial_prover]
+name = "Alt-Ergo"
+path = "/home/rui/.opam/default/bin/alt-ergo"
+version = "2.5.4"
+
+[partial_prover]
+name = "CVC4"
+path = "/usr/local/bin/cvc4"
+version = "1.8"
+
+[partial_prover]
+name = "Coq"
+path = "/home/rui/.opam/default/bin/coqtop"
+version = "8.18.0"
+
+[partial_prover]
+name = "Z3"
+path = "/home/rui/.opam/default/bin/z3"
+version = "4.13.0"
+```
