proof/correctness/README.md
@@ -1,0 +1,29 @@
+## Notes
+
+|      op      | idx |
+|:------------:|:---:|
+| tree         | 1,2 |
+| type         |   3 |
+| ots          |   4 |
+| ltree        |   4 |
+| chain        |   5 |
+| tree height  |   5 |
+| tree idx     |   6 |
+| key and mask |   7 |
+
+
+## `#pre`
+
+```
+[wots_pkgen]: Changing index 5 of the address does not change the result
+[wots_pkgen]: Changing index 6 of the address does not change the result
+[wots_pkgen]: Changing index 7 of the address does not change the result
+
+[expand_seed]: Changing index 5 of the address does not change the result
+[expand_seed]: Changing index 6 of the address does not change the result
+[expand_seed]: Changing index 7 of the address does not change the result
+```
+
+## `post`
+
+
