test/address_properties/README.md
@@ -1,0 +1,35 @@
+# Address
+
+```
+==============================================================
+[gen chain inplace:]
+index 6 was changed: value = 9 // MIN (start + steps - 1, w - 1)
+index 7 was changed: value = 1
+==============================================================
+
+```
+
+```
+[expand_seed]: Changing index 5 of the address does not change the result
+[expand_seed]: Changing index 6 of the address does not change the result
+[expand_seed]: Changing index 7 of the address does not change the result
+
+[expand seed:]
+index 5 was changed: value = 66 // len - 1
+index 6 was changed: value = 0
+index 7 was changed: value = 0
+```
+
+```
+[l_tree]: Changing index 0 of the address changes the result
+[l_tree]: Changing index 1 of the address changes the result
+[l_tree]: Changing index 2 of the address changes the result
+[l_tree]: Changing index 3 of the address changes the result
+[l_tree]: Changing index 4 of the address changes the result
+[l_tree]: Changing index 5 of the address changes the result
+[l_tree]: Changing index 6 of the address changes the result
+[l_tree]: Changing index 7 of the address changes the result
+[l_tree:] index 5 was changed: value = 7
+[l_tree:] index 6 was changed: value = 0
+[l_tree:] index 7 was changed: value = 2
+```
